The Great Refactor

coq/Main.v
@@ -1,116 +1,202 @@
 Set Implicit Arguments.
 Require Import Coq.Arith.PeanoNat Strings.String Lists.List Lia Program.Equality.
+Require Import CSC.Sets.
 
 Ltac inv H := (inversion H; subst; clear H).
 
-Section Compositionality.
+Axiom Events : Set.
 
-Axiom Trace : Set.
+(** * Traces *)
+CoInductive Trace : Set :=
+| TCons (e : Events) (t : Trace) : Trace
+.
+(** * Abstract description of a Programming Language
 
-(* Set of traces *)
-Definition Property := Trace -> Prop.
-
-(* Set of sets of traces *)
-Definition Hyperproperty := Property -> Prop.
-
-(* Sets of hyperproperties *)
-Definition PClass := Hyperproperty -> Prop.
-
-
-(* Set Theory Stuff *)
-Definition el { A } (x : A) (C : A -> Prop) := C x.
-Notation "x '∈' A" := (el x A) (at level 50).
-
-Definition subset { A } (C1 C2 : A -> Prop) := forall x, x ∈ C1 -> x ∈ C2.
-Notation "A '⊆' B" := (subset A B) (at level 50).
-Notation "A '≡' B" := (A ⊆ B /\ B ⊆ A) (at level 50).
-Axiom set_ext : forall A, forall (X Y : A -> Prop), X ≡ Y -> X = Y.
-
-Definition intersect { A } (C1 C2 : A -> Prop) := forall x, x ∈ C1 /\ x ∈ C2.
-
-Axiom Intersection : forall A, forall (C1 C2 : A -> Prop), A -> Prop.
-Notation "A '∩' B" := (Intersection A B) (at level 50).
-Axiom IntroIntersect : forall A, forall (X Y : A -> Prop), forall x, x ∈ X -> x ∈ Y -> x ∈ (X ∩ Y).
-Axiom ElimIntersect : forall A, forall (X Y : A -> Prop), forall x, x ∈ (X ∩ Y) -> x ∈ X /\ x ∈ Y.
-
-
-Definition union { A } (C1 C2 : A -> Prop) := forall x, x ∈ C1 \/ x ∈ C2.
-
-Axiom Union : forall A, forall (C1 C2 : A -> Prop), A -> Prop.
-Notation "A '∪' B" := (Union A B) (at level 50).
-Axiom IntroUnion : forall A, forall (X Y : A -> Prop), forall x, x ∈ X \/ x ∈ Y -> x ∈ (X ∪ Y).
-Axiom ElimUnion : forall A, forall (X Y : A -> Prop), forall x, x ∈ (X ∪ Y) -> x ∈ X \/ x ∈ Y.
-
-
-Lemma self_intersect { A } (C : A -> Prop) :
-  C ∩ C = C.
-Proof.
-  apply set_ext; split; intros x H.
-  - apply ElimIntersect in H; apply H.
-  - apply IntroIntersect; trivial.
-Qed.
-
-Lemma self_union { A } (C : A -> Prop) :
-  C ∪ C = C.
-Proof.
-  apply set_ext; split; intros x H.
-  - apply ElimUnion in H as []; trivial.
-  - apply IntroUnion; left; trivial.
-Qed.
-
-Record Language :=
+  Programming languages consist of:
+    - A set of (admissible) partial programs.
+      Basically, partial programs are syntactically and semantically correct.
+    - A judgement that checks whether a partial program is partial or not.
+      Only whole programs can be executed.
+    - A judgement that checks whether a partial program is a value (e.g. `42`).
+    - The linker is self-explanatory.
+    - The step relation, as mentioned before, works on whole programs.
+      Instead of directly emitting the behavior, we require languages to be defined
+      in a small-step like manner, which will allow us to combine languages later in
+      interesting ways.
+    - Lastly, there is a lemma any language must satisfy: Given a whole program,
+      it may perform a step to another whole program emitting an event or terminate
+      in a value.
+*)
+(** Unfortunately, Coq 8.14.1 seems to have some issues with regards to dependent pattern
+    matching that don't allow us to state the lemma as a property of the record.
+    Henceforth, we pose it as a variable. *)
+Record Language : Type :=
 {
   Partials : Set;
   whole : Partials -> Prop;
-  link : Partials -> Partials -> Partials;
-  step : forall (p : Partials), whole p -> Property;
+  value : Partials -> Prop;
+  link : Partials -> Partials -> option Partials;
+  steps : forall (p : Partials), whole p -> Trace -> Prop;
 }.
 
-(* Languages *)
-Definition Compiler (L0 L1 : Language) := Partials L0 -> Partials L1.
+Module PropSetM <: SetBase.
+  Definition A := Trace.
+End PropSetM.
+Module PropSet <: Sig := SetTheoryAbstract PropSetM.
 
-Notation "C '[' P ']'" := (link _ P C) (at level 50).
+Module HPropSetM <: SetBase.
+  Definition A := PropSet.set.
+End HPropSetM.
+Module HPropSet <: Sig := SetTheoryAbstract HPropSetM.
 
-Definition seqcomp {L0 L1 L2 : Language} (f : Compiler L1 L2) (g : Compiler L0 L1) := fun x => f (g x).
-Notation "f '∘' g" := (seqcomp g f) (at level 50).
+Module HPropClassM <: SetBase.
+  Definition A := HPropSet.set.
+End HPropClassM.
+Module HPropClass <: Sig := SetTheoryAbstract HPropClassM.
 
+(** Set of traces. *)
+Definition Property := PropSet.set.
+
+(** Set of sets of traces. *)
+Definition Hyperproperty := HPropSet.set.
+
+(** Sets of hyperproperties *)
+Definition PClass := HPropClass.set.
+
+Notation "C '⋈' P" := (link _ P C) (at level 50).
 Section Satisfaction.
 
+(** * Different kinds of Satisfaction Criteria *)
 Context {K : Language}.
 
-Definition sat (p : Partials K) (π : Property) : Prop := forall (H : whole K p), forall t, step K p H t -> t ∈ π.
-Definition rsat (p : Partials K) (π : Property) : Prop := forall (c : Partials K), sat (c[p]) π.
+Definition behav (p : Partials K) (H : whole K p) : HPropSet.A :=
+  fun (t : Trace) => steps K p H t.
 
-Definition behaviour (p : Partials K) (H : whole K p) : Property := fun b => step K p H b.
+Section A.
+Import HPropSet HPropSet.Notations.
+Definition hsat (p : Partials K) (Π : Hyperproperty) : Prop :=
+  forall (H : whole K p), HPropSet.el (behav p H) Π.
+End A.
+Section A.
+(* TODO: notation of sets should somehow work on a typeclass*)
+Import HPropSet HPropSet.Notations.
+Definition subset_closed (Π : Hyperproperty) :=
+  forall (π : Property), π ∈ Π -> forall (π' : Property), PropSet.subset π' π -> π' ∈ Π.
+End A.
+Definition rhsat (p : Partials K) (Π : Hyperproperty) : Prop :=
+  forall (c : Partials K),
+    match (c ⋈ p) with
+    | None => False
+    | Some L => hsat L Π
+    end.
 
-Definition hsat (p : Partials K) (Π : Hyperproperty) : Prop := forall (H : whole K p), behaviour p H ∈ Π.
-Definition rhsat (p : Partials K) (Π : Hyperproperty) : Prop := forall (c : Partials K), hsat (c[p]) Π.
-
+Import HPropClass HPropClass.Notations.
 Definition csat (p : Partials K) (C : PClass) : Prop := forall Π, Π ∈ C -> hsat p Π.
 Definition rcsat (p : Partials K) (C : PClass) : Prop := forall Π, Π ∈ C -> rhsat p Π.
 
 End Satisfaction.
 
+Definition SumLanguage (L0 L1 : Language)
+           (cross_linker : Partials L0 -> Partials L1 -> option (Partials L0 + Partials L1))
+  :=
+{|
+  Partials := Partials L0 + Partials L1 ;
+  whole := fun (p : Partials L0 + Partials L1) =>
+             match p with
+             | inl p0 => whole L0 p0
+             | inr p1 => whole L1 p1
+             end
+          ;
+  value := fun (p : Partials L0 + Partials L1) =>
+             match p with
+             | inl p0 => value L0 p0
+             | inr p1 => value L1 p1
+             end
+          ;
+  link := fun (p0 p1 : Partials L0 + Partials L1) =>
+            match p0, p1 with
+            | inl pa, inl pb => match (link L0 pa pb) with
+                               | Some L => Some(inl L)
+                               | None => None
+                               end
+            | inr pa, inr pb => match (link L1 pa pb) with
+                               | Some L => Some(inr L)
+                               | None => None
+                               end
+            | inl pa, inr pb => cross_linker pa pb
+            | inr pa, inl pb => cross_linker pb pa
+            end
+          ;
+  steps := fun p =>
+            match p with
+            | inl p0 => (fun (H' : whole L0 p0) => steps L0 p0 H')
+            | inr p1 => (fun (H' : whole L1 p1) => steps L1 p1 H')
+            end
+          ;
+|}.
+Definition ProdLanguage (L0 L1 : Language) :=
+{|
+  Partials := (Partials L0) * (Partials L1) ;
+  whole := fun (p : (Partials L0) * (Partials L1)) =>
+             match p with
+             | (p0, p1) => whole L0 p0 /\ whole L1 p1
+             end
+           ;
+  value := fun (p : (Partials L0) * (Partials L1)) =>
+             match p with
+             | (p0, p1) => value L0 p0 /\ value L1 p1
+             end
+           ;
+  link := fun (p0 p1 : (Partials L0) * (Partials L1)) =>
+            match p0, p1 with
+            | (pa0, pa1), (pb0, pb1) =>
+                match link L0 pa0 pb0, link L1 pa1 pb1 with
+                | Some A, Some B => Some (A,B)
+                | _, _ => None
+                end
+            end
+          ;
+  steps := fun p =>
+            let '(p0a, p1a) := p in
+            fun H =>
+            match H with
+            | conj H0a H1a => fun t => steps L0 p0a H0a t /\ steps L1 p1a H1a t
+            end
+          ;
+|}.
+Notation "L0 'L*' L1" := (ProdLanguage L0 L1) (at level 80).
+
+
+(** * Compilers *)
+Definition Compiler (L0 L1 : Language) := Partials L0 -> Partials L1.
+
+Definition seqcomp {L0 L1 L2 : Language} (f : Compiler L1 L2) (g : Compiler L0 L1) := fun x => f (g x).
+Notation "f '∘' g" := (seqcomp g f) (at level 50).
+
 Notation "p '|-' C" := (rcsat p C) (at level 50).
 Notation "p '|=' Π" := (rhsat p Π) (at level 50).
-
-Lemma weakening_rcsat { K : Language } C1 C2 (p : Partials K) :
-  C1 ⊆ C2 -> p |- C2 -> p |- C1.
-Proof.
-  intros H H0 Π H1; apply H0, H, H1.
-Qed.
 
 Section Main.
 
 Variable S I T : Language.
+Variable linkSI : Partials S -> Partials I -> option (Partials S + Partials I).
 
-(* Robust Compilation *)
+(** * Property mappings *)
+(** Given must be a relation between traces of a source and a target language. *)
+
+(** TODO: Add ext. image and all that. See
+    https://github.com/secure-compilation/different_traces/blob/master/SSCHPreservation.v *)
+
+Import HPropClass HPropClass.Notations.
 Definition RC { L0 L1 : Language } (γ : Compiler L0 L1) (C : PClass) :=
-  forall Π, Π ∈ C -> forall (p : Partials L0), p |= Π -> γ p |= Π.
-Notation "'|-' γ ':' C" := (RC γ C) (at level 50, γ at next level).
+  forall (Π : Hyperproperty), Π ∈ C ->
+    forall (p : Partials L0), p |= Π -> γ p |= Π.
+Notation "'pres|-' γ ':' C" := (RC γ C) (at level 50, γ at next level).
 
-Lemma seqcomp_compose (γ0 : Compiler S I) (γ1 : Compiler I T) (C0 C1 : PClass) :
-  |- γ0 : C0 -> |- γ1 : C1 -> |- (γ0 ∘ γ1) : (C0 ∩ C1).
+(** * Main Results *)
+
+Lemma sequential_composition (γ0 : Compiler S I) (γ1 : Compiler I T) (C0 C1 : PClass) :
+  pres|- γ0 : C0 -> pres|- γ1 : C1 -> pres|- (γ0 ∘ γ1) : (C0 ∩ C1).
 Proof.
   intros H0 H1 Π H2 p H3.
   apply ElimIntersect in H2 as [H2a H2b].
@@ -119,7 +205,7 @@ Proof.
 Qed.
 
 Corollary swappable (γ0 γ1 : Compiler I I) (C0 C1 : PClass) :
-  |- γ0 : C0 -> |- γ1 : C1 -> |- (γ0 ∘ γ1) : (C0 ∩ C1) /\ |- (γ1 ∘ γ0) : (C0 ∩ C1).
+  pres|- γ0 : C0 -> pres|- γ1 : C1 -> pres|- (γ0 ∘ γ1) : (C0 ∩ C1) /\ pres|- (γ1 ∘ γ0) : (C0 ∩ C1).
 Proof.
   intros H0 H1; split.
   all:
@@ -128,28 +214,160 @@ Proof.
   (apply H1, H0 || apply H0, H1); trivial.
 Qed.
 
-Lemma weakening_RC (γ : Compiler S T) (C0 C1 : PClass) :
-  C0 ⊆ C1 -> |- γ : C1 -> |- γ : C0.
+Definition UpperComposition { L0 L1 L2 : Language } { cross_link }
+    (γ0 : Compiler L0 L2) (γ1 : Compiler L1 L2)
+  : Partials (SumLanguage L0 L1 cross_link) -> Partials L2
+  :=
+  fun (pab : Partials (SumLanguage L0 L1 cross_link)) =>
+    match pab with
+    | inl p => γ0 p
+    | inr p => γ1 p
+    end
+.
+Lemma upper_compose (γ0 : Compiler S T) (γ1 : Compiler I T) (C0 C1 : PClass) :
+  pres|- γ0 : C0 -> pres|- γ1 : C1 -> pres|- (@UpperComposition S I T linkSI γ0 γ1) : (C0 ∩ C1).
 Proof.
-  intros H0 H1 Π H2 p H3.
-  apply H1; trivial.
-  apply H0; trivial.
-Qed.
+  intros H0 H1 Π H2 [pS | pI] H3; apply ElimIntersect in H2 as [H2a H2b].
+  - apply H0; try easy.
+    intros Cs; specialize (H3 (inl Cs)).
+    (* exact H3. *)
+    (** This doesn't work out, since programs in the SumLang might go from S to I
+        in intermediate steps. *)
+    admit.
+  - apply H1; try easy.
+    intros Cs; specialize (H3 (inr Cs)).
+    (* exact H3. *)
+    (** Same business. *)
+    admit.
+Admitted.
+(* Secure Enforcements *)
+Definition enforcement { L0 L1 : Language } (γ : Compiler L0 L1) (C : PClass) := forall (p : Partials L0), rcsat (γ p) C.
+Notation "'enf|-' γ '--≻' C" := (enforcement γ C) (at level 80).
 
-(* Secure Instrumentations *)
-Definition instrumentation { L0 L1 : Language } (γ : Compiler L0 L1) (C : PClass) := forall (p : Partials L0), rcsat (γ p) C.
-Definition secure_instrumentation { L0 L1 : Language } (γ : Compiler L0 L1) (C0 C1 : PClass) := |- γ : C0 /\ instrumentation γ C1.
-Notation "γ '-' C0 '-≻' C1" := (secure_instrumentation γ C0 C1) (at level 50).
+Definition secure_enforcement { L0 L1 : Language } (γ : Compiler L0 L1) (C0 C1 : PClass) :=
+  pres|- γ : C0 /\ enf|- γ --≻ C1.
+Notation "'senf|-' γ '-[' C0 ']-≻' C1" := (secure_enforcement γ C0 C1) (at level 50).
 
-Lemma glue (γ0 : Compiler S I) (γ1 : Compiler I T) (C0 C1 : PClass) :
-  |- γ0 : C0 -> γ1 -C0-≻ C1 -> |- (γ0 ∘ γ1) : (C0 ∪ C1).
+Lemma senf_and_rc (γ0 : Compiler S I) (γ1 : Compiler I T) (C0 C1 : PClass) :
+  pres|- γ0 : C0 -> senf|- γ1 -[ C0 ]-≻ C1 -> pres|- (γ0 ∘ γ1) : (C0 ∪ C1).
 Proof.
   intros H0 [H1a H1b] Π H2 p H3.
   apply ElimUnion in H2 as [H2a|H2b].
-  - eapply seqcomp_compose; eauto; rewrite self_intersect; trivial.
-  - apply H1b, H2b.
+  - apply H1a; trivial. apply H0; trivial.
+  - apply H1b; trivial.
+Qed.
+
+Lemma rc_and_senf (γ0 : Compiler S I) (γ1 : Compiler I T) (C0 C1 : PClass) :
+  senf|- γ0 -[ C0 ]-≻ C1 -> pres|- γ1 : C0 -> pres|- (γ0 ∘ γ1) : (C0 ∪ C1).
+Proof.
+  intros [H0a H0b] H1 Π H2 p H3.
+  apply ElimUnion in H2 as [H2a|H2b].
+  - apply H1; trivial. apply H0a; trivial.
+  - (** This is where things go wrong. We can only apply H1, but this means
+        we need to prove that our pi is in C0, which it isn't...!           *)
+Abort.
+
+(** * Bonus *)
+
+Lemma join_sinstrus (γ1 : Compiler S I) (γ2 : Compiler I T) (C0 C1 C2 : PClass) :
+  senf|- γ1 -[C0]-≻ C1 -> senf|- γ2 -[C1]-≻ C2 -> senf|- (γ1 ∘ γ2) -[C0 ∩ C1]-≻ (C1 ∪ C2).
+Proof.
+  intros [H0a H0b] [H1a H1b]; split.
+  - intros Π H2 p H3; apply ElimIntersect in H2 as [H2a H2b].
+    apply H1a; trivial; apply H0a; trivial.
+  - intros p Π H2; apply ElimUnion in H2 as [H2a|H2b].
+    + apply H1a; trivial; now apply H0b.
+    + now apply H1b.
+Qed.
+
+Lemma instru_union (γ : Compiler S T) (C0 C1 : PClass) :
+  senf|- γ -[C0]-≻ C1 -> pres|- γ : (C0 ∪ C1).
+Proof.
+  intros [H0a H0b] Π H2 p H3.
+  apply ElimUnion in H2 as [H2a|H2b].
+  - apply H0a; assumption.
+  - apply H0b; assumption.
+Qed.
+Lemma instru_cap (γ : Compiler S T) (C0 C1 : PClass) :
+  senf|- γ -[C0]-≻ C1 -> pres|- γ : (C0 ∩ C1).
+Proof.
+  intros [H0a H0b] Π H2 p H3.
+  apply ElimIntersect in H2 as [H2a H2b].
+  now apply H0a.
+Qed.
+
+Lemma join_instrus (γ0 : Compiler S I) (γ1 : Compiler I T) (C0 C1 : PClass) :
+  senf|- γ0 -[C1]-≻ C0 -> senf|- γ1 -[C0]-≻ C1 -> senf|- (γ0 ∘ γ1) -[C1]-≻ C0 /\ senf|- (γ0 ∘ γ1) -[C0]-≻ C1.
+Proof.
+  intros [H0a H0b] [H1a H1b]; repeat split.
+  - intros Π H2 p H3. now apply H1b.
+  - intros p Π H2. apply H1a; try assumption. now apply H0b.
+  - intros Π H2 p H3. apply H1a; try assumption. now apply H0b.
+  - intros p Π H2. now apply H1b.
+Qed.
+
+Lemma swappable_instrus (γ0 : Compiler I I) (γ1 : Compiler I I) (C0 C1 : PClass) :
+  senf|- γ0 -[C0]-≻ C1 -> senf|- γ1 -[C1]-≻ C0 -> senf|- (γ0 ∘ γ1) -[C0 ∪ C1]-≻ (C0 ∪ C1) /\
+                                              senf|- (γ1 ∘ γ0) -[C0 ∪ C1]-≻ (C0 ∪ C1).
+Proof.
+  intros [H0a H0b] [H1a H1b]; repeat split.
+  - intros Π H2 p H3; apply ElimUnion in H2 as [H2a|H2b].
+    + now apply H1b.
+    + apply H1a; trivial; now apply H0b.
+  - intros p Π H2; apply ElimUnion in H2 as [H2a|H2b].
+    + now apply H1b.
+    + apply H1a; trivial; now apply H0b.
+  - intros Π H2 p H3; apply ElimUnion in H2 as [H2a|H2b].
+    + apply H0a; trivial; now apply H1b.
+    + now apply H0b.
+  - intros p Π H2; apply ElimUnion in H2 as [H2a|H2b].
+    + apply H0a; trivial; now apply H1b.
+    + now apply H0b.
+Qed.
+
+
+(* Lower Composition *)
+Definition LowerComposition { L0 L1 L2 : Language } (γ0 : Compiler L0 L1) (γ1 : Compiler L0 L2)
+  : Partials L0 -> Partials (ProdLanguage L1 L2)
+  :=
+  fun (p : Partials L0) => (γ0 p, γ1 p)
+.
+
+Definition ssc_class (C : PClass) :=
+  forall (Π : Hyperproperty), Π ∈ C -> subset_closed Π.
+
+Lemma lowercomp_compose (γ0 : Compiler S I) (γ1 : Compiler S T) (C0 C1 : PClass) :
+  ssc_class C0 ->
+  pres|- γ0 : C0 -> pres|- γ1 : C1 -> pres|- (LowerComposition γ0 γ1) : (C0 ∩ C1).
+Proof.
+  intros SSC0 H0 H1 Π H2 p H3; apply ElimIntersect in H2 as [H2a H2b].
+  intros [Ci Ct]. unfold LowerComposition in *.
+  apply H0 in H3 as H3a; apply H1 in H3 as H3b; trivial.
+  unfold "_ |= _" in *.
+  admit. (*
+  unfold behaviour; cbn; destruct Hw as [Hw0 Hw1].
+  specialize (H3a Ci Hw0); specialize (H3b Ct Hw1).
+  unfold behaviour in H3a, H3b.
+  change (fun b => ?h b) with h in H3a, H3b.
+  apply SSC0 in H2a as SSPi. eapply SSPi in H3a, H3b.
+  apply H3a. intros τ H4.
+  change (τ ∈ (fun b : Trace => ?h b)) with (τ ∈ h) in H4.
+  unfold "_ ∈ _" in *. destruct H4 as [H4a H4b]. assumption.
+  *)
+Admitted.
+
+Lemma enforcement_implies_robustness (γ : Compiler S I) (C : PClass) :
+  enf|- γ --≻ C -> pres|- γ : C.
+Proof.
+  intros H0 Π H1 p H2; now apply H0.
+Qed.
+
+Lemma enforcements_are_secure_for_fixed_class (γ : Compiler S I) (C : PClass) :
+  enf|- γ --≻ C -> senf|- γ -[C]-≻ C.
+Proof.
+  intros H0; split.
+  - intros H1 Π H2 p; now apply H0.
+  - exact H0.
 Qed.
 
 End Main.
-End Compositionality.
-
